serialize DER lengths (we forgot nothing)

src/lowparse/LowParse.Spec.DER.fst
@@ -1,15 +1,15 @@
 module LowParse.Spec.DER
 include LowParse.Spec.Combinators
-include LowParse.Spec.Bytes
+include LowParse.Spec.SeqBytes
 
 include LowParse.Spec.Int
 open FStar.Mul
 
-module B32 = FStar.Bytes
 module U8 = FStar.UInt8
 module UInt = FStar.UInt
 module Math = LowParse.Math
 module E = LowParse.BigEndian
+module Seq = FStar.Seq
 
 #reset-options "--z3cliopt smt.arith.nl=false --max_fuel 0 --max_ifuel 0"
 
@@ -64,10 +64,10 @@ let tag_of_der_length
 
 let synth_be_int
   (len: nat)
-  (b: B32.lbytes len)
+  (b: Seq.lseq byte len)
 : GTot (x: nat { x < pow2 (8 * len) })
-= E.lemma_be_to_n_is_bounded (B32.reveal b);
-  E.be_to_n (B32.reveal b)
+= E.lemma_be_to_n_is_bounded b;
+  E.be_to_n b
 
 let synth_be_int_injective
   (len: nat)
@@ -75,9 +75,39 @@ let synth_be_int_injective
   (synth_injective (synth_be_int len))
   [SMTPat (synth_injective (synth_be_int len))]
 = 
-  synth_injective_intro' (synth_be_int len) (fun (x x' : B32.lbytes len) ->
-    E.be_to_n_inj (B32.reveal x) (B32.reveal x')
+  synth_injective_intro' (synth_be_int len) (fun (x x' : Seq.lseq byte len) ->
+    E.be_to_n_inj x x'
   )
+
+let synth_der_length_129
+  (x: U8.t { x == 129uy } )
+  (y: U8.t { U8.v y >= 128 } )
+: GTot (refine_with_tag tag_of_der_length x)
+= assert_norm (der_length_max == pow2 (8 * 126) - 1);
+  assert_norm (pow2 7 == 128);
+  assert_norm (pow2 8 == 256);
+  assert_norm (256 < der_length_max);
+  assert (U8.v x <= der_length_max);
+  log256_unique (U8.v y) 1;
+  U8.v y
+
+let synth_der_length_greater
+  (x: U8.t { U8.v x > 129 /\ U8.v x < 255 } )
+  (len: nat { len == U8.v x % 128 } )
+  (y: (y: nat { y < pow2 (8 * len) } ) { y >= pow2 (8 * (len - 1)) } )
+: Tot (refine_with_tag tag_of_der_length x)
+= assert_norm (der_length_max == pow2 (8 * 126) - 1);
+  assert_norm (pow2 7 == 128);
+  assert_norm (pow2 8 == 256);
+  assert_norm (256 < der_length_max);
+  assert (U8.v x <= der_length_max);
+  Math.lemma_mod_lt (U8.v x) (pow2 7);
+  Math.lemma_div_mod (U8.v x) (pow2 7);
+  Math.division_definition (U8.v x) (pow2 7) 1;
+  Math.pow2_le_compat (8 * 126) (8 * len);
+  Math.pow2_le_compat (8 * (len - 1)) 7;
+  log256_unique y len;
+  y
 
 let parse_der_length_payload
   (x: U8.t)
@@ -102,25 +132,14 @@ let parse_der_length_payload
    then
     weaken parse_der_length_payload_kind
       ((parse_u8 `parse_filter` (fun y -> U8.v y >= 128))
-        `parse_synth` (fun (y: U8.t { U8.v y >= 128 } ) -> (
-          log256_unique (U8.v y) 1;
-          U8.v y <: refine_with_tag tag_of_der_length x
-      )))
+        `parse_synth` synth_der_length_129 x)
   else begin
-    let len = U8.v x % pow2 7 in
-    Math.lemma_mod_lt (U8.v x) (pow2 7);
-    Math.lemma_div_mod (U8.v x) (pow2 7);
-    Math.division_definition (U8.v x) (pow2 7) 1;
-    Math.pow2_le_compat (8 * 126) (8 * len);
-    Math.pow2_le_compat (8 * (len - 1)) 7;
-    synth_be_int_injective len;
+    let len : nat = U8.v x % pow2 7 in
+    synth_be_int_injective len; // FIXME: WHY WHY WHY does the pattern not trigger, even with higher rlimit?
     weaken parse_der_length_payload_kind
-      (((parse_flbytes len `parse_synth` (synth_be_int len))
+      (((parse_seq_flbytes len `parse_synth` (synth_be_int len))
         `parse_filter` (fun (y: nat { y < pow2 (8 * len) } ) -> y >= pow2 (8 * (len - 1))))
-       `parse_synth` (fun (y: (y: nat { y < pow2 (8 * len) } ) { y >= pow2 (8 * (len - 1)) } ) ->
-         log256_unique y len;
-         y <: refine_with_tag tag_of_der_length x
-      ))
+       `parse_synth` synth_der_length_greater x len)
   end        
         
 inline_for_extraction
@@ -131,3 +150,124 @@ let parse_der_length : parser parse_der_length_kind der_length_t
     parse_u8
     tag_of_der_length
     parse_der_length_payload
+
+let tag_of_der_length_lt_128
+  (x: der_length_t)
+: Lemma
+  (requires (U8.v (tag_of_der_length x) < 128))
+  (ensures (x == U8.v (tag_of_der_length x)))
+= if x < 128
+  then ()
+  else
+    let len_len = log256 x in
+    assert_norm (der_length_max == pow2 (8 * 126) - 1);
+    Math.pow2_lt_recip (8 * (len_len - 1)) (8 * 126)
+
+let tag_of_der_length_invalid
+  (x: der_length_t)
+: Lemma
+  (requires (let y = U8.v (tag_of_der_length x) in y == 128 \/ y == 255))
+  (ensures False)
+= if x < 128
+  then ()
+  else
+    let len_len = log256 x in
+    assert_norm (der_length_max == pow2 (8 * 126) - 1);
+    Math.pow2_lt_recip (8 * (len_len - 1)) (8 * 126)
+
+let tag_of_der_length_eq_129
+  (x: der_length_t)
+: Lemma
+  (requires (U8.v (tag_of_der_length x) == 129))
+  (ensures (x >= 128 /\ x < 256))
+= if x < 128
+  then ()
+  else
+    let len_len = log256 x in
+    assert_norm (der_length_max == pow2 (8 * 126) - 1);
+    Math.pow2_lt_recip (8 * (len_len - 1)) (8 * 126)
+
+let synth_der_length_129_recip
+  (x: U8.t { x == 129uy })
+  (y: refine_with_tag tag_of_der_length x)
+: GTot (y: U8.t {U8.v y >= 128})
+= tag_of_der_length_eq_129 y;
+  U8.uint_to_t y
+
+let synth_be_int_recip
+  (len: nat)
+  (x: nat { x < pow2 (8 * len) })
+: GTot (b: Seq.lseq byte len)
+= E.n_to_be'' len x
+
+let synth_be_int_inverse
+  (len: nat)
+: Lemma
+  (synth_inverse (synth_be_int len) (synth_be_int_recip len))
+= ()
+
+let synth_der_length_greater_recip
+  (x: U8.t { U8.v x > 129 /\ U8.v x < 255 } )
+  (len: nat { len == U8.v x % 128 } )
+  (y: refine_with_tag tag_of_der_length x)
+: Tot (y: (y: nat { y < pow2 (8 * len) } ) { y >= pow2 (8 * (len - 1)) } )
+= assert_norm (der_length_max == pow2 (8 * 126) - 1);
+  Math.pow2_lt_recip (8 * (log256 y - 1)) (8 * 126);
+  y
+
+let synth_der_length_greater_inverse
+  (x: U8.t { U8.v x > 129 /\ U8.v x < 255 } )
+  (len: nat { len == U8.v x % 128 } )
+: Lemma
+  (synth_inverse (synth_der_length_greater x len) (synth_der_length_greater_recip x len))
+= ()
+
+let serialize_der_length_payload
+  (x: U8.t)
+: Tot (serializer (parse_der_length_payload x))
+= assert_norm (der_length_max == pow2 (8 * 126) - 1);
+  assert_norm (pow2 7 == 128);
+  assert_norm (pow2 8 == 256);
+  assert_norm (256 < der_length_max);
+  assert (U8.v x <= der_length_max);
+  let (x' : der_length_t) = U8.v x in
+  if x' < 128
+  then begin
+    serialize_weaken parse_der_length_payload_kind (serialize_ret (x' <: refine_with_tag tag_of_der_length x) (fun (y: refine_with_tag tag_of_der_length x) -> tag_of_der_length_lt_128 y))
+  end else
+   if x = 128uy || x = 255uy
+   then
+     fail_serializer parse_der_length_payload_kind (refine_with_tag tag_of_der_length x) (fun y -> tag_of_der_length_invalid y)
+   else if x = 129uy
+   then begin
+     serialize_weaken
+       parse_der_length_payload_kind
+       (serialize_synth
+          (parse_filter parse_u8 (fun y -> U8.v y >= 128))
+          (synth_der_length_129 x)
+          (serialize_filter serialize_u8 (fun y -> U8.v y >= 128))
+          (synth_der_length_129_recip x)
+          (synth_inverse_intro' (synth_der_length_129 x) (synth_der_length_129_recip x) (fun (y: refine_with_tag tag_of_der_length x) -> tag_of_der_length_eq_129 y))
+       )
+   end else begin
+    let len : nat = U8.v x % pow2 7 in
+    synth_be_int_injective len; // FIXME: WHY WHY WHY does the pattern not trigger, even with higher rlimit?
+    serialize_weaken
+      parse_der_length_payload_kind
+      (serialize_synth
+        _
+        (synth_der_length_greater x len)
+        (serialize_filter
+          (serialize_synth
+            _
+            (synth_be_int len)
+            (serialize_seq_flbytes len)
+            (synth_be_int_recip len)
+            ()
+          )
+          (fun (y: nat { y < pow2 (8 * len) } ) -> y >= pow2 (8 * (len - 1)))
+        )
+        (synth_der_length_greater_recip x len)
+        ()
+      )
+   end
